move some things to more logical places

theories/simulation/simulation.v
@@ -1,37 +1,19 @@
+(** Notational typeclasses for simulation relations. *)
 
-From iris.bi Require Import bi lib.fixpoint.
-From iris.prelude Require Import prelude.
-From iris.proofmode Require Import tactics.
+From iris.bi Require Import bi.
 From simuliris.simulation Require Import relations language.
 From iris.prelude Require Import options.
 Import bi.
 
-(* parameterized over "external" relation that restricts values passed to and
-from external function calls *)
-(* TODO: Hint Mode? *)
-Class simulirisGS (PROP : bi) (Λ : language) := SimulirisGS {
-  (* state interpretation *)
-  state_interp : prog Λ → state Λ → prog Λ → state Λ → list (expr Λ) → PROP;
-  state_interp_pure_prim_step P_t σ_t P_s σ_s e_s T π e_s':
-    T !! π = Some e_s →
-    (∀ σ_s, prim_step P_s e_s σ_s e_s' σ_s []) →
-    state_interp P_t σ_t P_s σ_s T -∗
-    state_interp P_t σ_t P_s σ_s (<[π:=e_s']>T);
-  (* external function call relation *)
-  ext_rel : thread_id → val Λ → val Λ → PROP;
-}.
-
 (** Typeclass for the simulation relation so we can use the definitions with
    greatest+least fp (stuttering) or just greatest fp (no stuttering). *)
-Class Sim (PROP : bi) (Λ : language) {s : simulirisGS PROP Λ} :=
+Class Sim (PROP : bi) (Λ : language) :=
   sim : (val Λ → val Λ → PROP) → thread_id → expr Λ → expr Λ → PROP.
-#[global]
-Hint Mode Sim - - - : typeclass_instances.
+(* We assume only one instance is ever in scope, hence no mode *)
 
-Class SimE (PROP : bi) (Λ : language) {s : simulirisGS PROP Λ} :=
+Class SimE (PROP : bi) (Λ : language) :=
   sim_expr : (expr Λ → expr Λ → PROP) → thread_id → expr Λ → expr Λ → PROP.
-#[global]
-Hint Mode SimE - - - : typeclass_instances.
+(* We assume only one instance is ever in scope, hence no mode *)
 
 (* FIXME what are good levels for et, es? *)
 Notation "et '⪯{' π '}' es {{ Φ }}" := (sim Φ π et es) (at level 40, Φ at level 200,
@@ -40,35 +22,6 @@ Notation "et '⪯{' π '}' es {{ Φ }}" := (sim Φ π et es) (at level 40, Φ at
 (* FIXME: the notation with binder doesn't work; left-factoring seems to fail.
 Notation "et  '⪯'  es  {{  v_t  v_s ,  P  }}" := (sim et es (λ v_t v_s, P)) (at level 40, v_t, v_s at level 200, P at level 200) : bi_scope. *)
 
-
 (* TODO: different symbols (no brackets) for expr thing *)
 Notation "et '⪯{' π '}' es [{ Φ }]" := (sim_expr Φ π et es) (at level 40, Φ at level 200,
   format "et  '⪯{' π '}'  es  [{  Φ  }]") : bi_scope.
-
-
-
-Section fix_lang.
-  Context {PROP : bi}.
-  Context {Λ : language}.
-  Context `{!simulirisGS PROP Λ}.
-
-  Definition progs_are (P_t P_s : prog Λ) : PROP :=
-    (□ ∀ P_t' P_s' σ_t σ_s T_s, state_interp P_t' σ_t P_s' σ_s T_s → ⌜P_t' = P_t⌝ ∧ ⌜P_s' = P_s⌝)%I.
-
-  Global Instance progs_are_persistent (P_s P_t : prog Λ) :
-    Persistent (progs_are P_s P_t).
-  Proof. rewrite /progs_are; apply _. Qed.
-
-  (** Lift simulation to whole-program relation *)
-  Definition prog_rel `{!Sim PROP Λ} (P_t P_s : prog Λ) : PROP :=
-    (□ ∀ f x_s e_s, ⌜P_s !! f = Some (x_s, e_s)⌝ →
-       ∃ x_t e_t, ⌜P_t !! f = Some (x_t, e_t)⌝ ∗
-         ∀ v_t v_s π, ext_rel π v_t v_s -∗
-           (subst_map {[x_t:=v_t]} e_t) ⪯{π} (subst_map {[x_s:=v_s]} e_s) {{ ext_rel π }})%I.
-
-  Global Instance prog_rel_persistent `{!Sim PROP Λ} P_t P_s : Persistent (prog_rel P_t P_s).
-  Proof. rewrite /prog_rel; apply _. Qed.
-End fix_lang.
-
-Global Hint Mode progs_are - - - + + : typeclass_instances.
-Typeclasses Opaque prog_rel.
