theories/stacked_borrows/steps_refl.v
@@ -4,7 +4,7 @@ From simuliris.base_logic Require Export gen_sim_prog.
 From simuliris.simulation Require Export slsls.
 From simuliris.simulation Require Import lifting.
 From simuliris.stacked_borrows Require Import tkmap_view.
-From simuliris.stacked_borrows Require Export defs.
+From simuliris.stacked_borrows Require Export defs class_instances.
 From simuliris.stacked_borrows Require Import steps_progress steps_retag steps_inv.
 From simuliris.stacked_borrows Require Import logical_state inv_accessors.
 From iris.prelude Require Import options.
